compiles and proof checks

w64x4/proof/Fp_w64x4_extract.ec
@@ -1,45 +1,30 @@
 require import AllCore IntDiv CoreMap List Distr.
-require import JModel.
+from Jasmin require import JModel.
 
-require import Array4 Array8.
-require import WArray32 WArray64.
+require import Array4.
+require import WArray32.
 
 
 
 module M = {
-  proc bn2_unpack (a:W64.t Array8.t) : W64.t Array4.t * W64.t Array4.t = {
+  proc bn_subc (a:W64.t Array4.t, b:W64.t Array4.t) : bool * W64.t Array4.t = {
     var aux: int;
     
-    var hi:W64.t Array4.t;
-    var lo:W64.t Array4.t;
-    var i:int;
-    hi <- witness;
-    lo <- witness;
-    i <- 0;
-    while (i < 4) {
-      lo.[i] <- a.[i];
-      hi.[i] <- a.[(4 + i)];
-      i <- i + 1;
-    }
-    return (hi, lo);
-  }
-  
-  proc bn_add1 (a:W64.t Array4.t, b:W64.t) : bool * W64.t Array4.t = {
-    var aux: bool;
-    var aux_1: int;
-    var aux_0: W64.t;
-    
     var cf:bool;
+    var x1:W64.t;
+    var x2:W64.t;
     var i:int;
     
-    (aux, aux_0) <- addc_64 a.[0] b false;
-    cf <- aux;
-    a.[0] <- aux_0;
+    x1 <- a.[0];
+    x2 <- b.[0];
+    (cf, x1) <- sbb_64 x1 x2 false;
+    a.[0] <- x1;
     i <- 1;
     while (i < 4) {
-      (aux, aux_0) <- addc_64 a.[i] (W64.of_int 0) cf;
-      cf <- aux;
-      a.[i] <- aux_0;
+      x1 <- a.[i];
+      x2 <- b.[i];
+      (cf, x1) <- sbb_64 x1 x2 cf;
+      a.[i] <- x1;
       i <- i + 1;
     }
     return (cf, a);
@@ -55,124 +40,17 @@ module M = {
     
     x1 <- a.[0];
     x2 <- b.[0];
-    (cf, x1) <- addc_64 x1 x2 false;
+    (cf, x1) <- adc_64 x1 x2 false;
     a.[0] <- x1;
     i <- 1;
     while (i < 4) {
       x1 <- a.[i];
       x2 <- b.[i];
-      (cf, x1) <- addc_64 x1 x2 cf;
+      (cf, x1) <- adc_64 x1 x2 cf;
       a.[i] <- x1;
       i <- i + 1;
     }
     return (cf, a);
-  }
-  
-  proc mul1 (a:W64.t, b:W64.t Array4.t) : W64.t * bool * bool *
-                                          W64.t Array8.t = {
-    var aux: int;
-    
-    var _zero:W64.t;
-    var of_0:bool;
-    var cf:bool;
-    var r:W64.t Array8.t;
-    var x1:W64.t;
-    var x2:W64.t;
-    var i:int;
-    var lo:W64.t;
-    var  _0:bool;
-    var  _1:bool;
-    var  _2:bool;
-    r <- witness;
-    (of_0, cf,  _0,  _1,  _2, _zero) <- set0_64 ;
-    x1 <- a;
-    x2 <- b.[0];
-    (x1, x2) <- MULX_64 x1 x2;
-    r.[1] <- x1;
-    r.[0] <- x2;
-    i <- 1;
-    while (i < 4) {
-      x1 <- a;
-      x2 <- b.[i];
-      (x1, x2) <- MULX_64 x1 x2;
-      r.[(i + 1)] <- x1;
-      lo <- x2;
-      x1 <- r.[i];
-      x2 <- lo;
-      (cf, x1) <- ADCX_64 x1 x2 cf;
-      r.[i] <- x1;
-      i <- i + 1;
-    }
-    x1 <- r.[4];
-    (cf, x1) <- ADCX_64 x1 _zero cf;
-    r.[4] <- x1;
-    return (_zero, of_0, cf, r);
-  }
-  
-  proc mul1acc (k:int, a:W64.t, b:W64.t Array4.t, r:W64.t Array8.t,
-                _zero:W64.t, of_0:bool, cf:bool) : W64.t * bool * bool *
-                                                   W64.t Array8.t = {
-    var aux: int;
-    
-    var x1:W64.t;
-    var i:int;
-    var x2:W64.t;
-    var hi:W64.t;
-    var lo:W64.t;
-    
-    aux <- (4 - 1);
-    i <- 0;
-    while (i < aux) {
-      x1 <- a;
-      x2 <- b.[i];
-      (x1, x2) <- MULX_64 x1 x2;
-      hi <- x1;
-      lo <- x2;
-      x1 <- r.[(k + i)];
-      (of_0, x1) <- ADOX_64 x1 lo of_0;
-      r.[(k + i)] <- x1;
-      x1 <- r.[((k + i) + 1)];
-      (cf, x1) <- ADCX_64 x1 hi cf;
-      r.[((k + i) + 1)] <- x1;
-      i <- i + 1;
-    }
-    x1 <- a;
-    x2 <- b.[(4 - 1)];
-    (x1, x2) <- MULX_64 x1 x2;
-    r.[(4 + k)] <- x1;
-    lo <- x2;
-    x1 <- r.[((4 + k) - 1)];
-    (of_0, x1) <- ADOX_64 x1 lo of_0;
-    r.[((4 + k) - 1)] <- x1;
-    x1 <- r.[(4 + k)];
-    (cf, x1) <- ADCX_64 x1 _zero cf;
-    r.[(4 + k)] <- x1;
-    x1 <- r.[(4 + k)];
-    (of_0, x1) <- ADOX_64 x1 _zero of_0;
-    r.[(4 + k)] <- x1;
-    return (_zero, of_0, cf, r);
-  }
-  
-  proc bn_muln (a:W64.t Array4.t, b:W64.t Array4.t) : W64.t * bool * bool *
-                                                      W64.t Array8.t = {
-    var aux: int;
-    
-    var _zero:W64.t;
-    var of_0:bool;
-    var cf:bool;
-    var r:W64.t Array8.t;
-    var ai:W64.t;
-    var i:int;
-    r <- witness;
-    ai <- a.[0];
-    (_zero, of_0, cf, r) <@ mul1 (ai, b);
-    i <- 1;
-    while (i < 4) {
-      ai <- a.[i];
-      (_zero, of_0, cf, r) <@ mul1acc (i, ai, b, r, _zero, of_0, cf);
-      i <- i + 1;
-    }
-    return (_zero, of_0, cf, r);
   }
   
   proc ith_bit64 (k:W64.t, ctr:W64.t) : W64.t = {
@@ -230,118 +108,57 @@ module M = {
     return (x, y);
   }
   
-  proc maskOnCarry (mask:int, r:W64.t, _cf:bool) : W64.t = {
+  proc cminusP (p:W64.t Array4.t, x:W64.t Array4.t) : W64.t Array4.t = {
     
-    
-    
-    (_cf, r) <- subc_64 r r _cf;
-    r <- (r `&` (W64.of_int mask));
-    return (r);
-  }
-  
-  proc cminusP (xx:W64.t Array4.t) : W64.t Array4.t = {
-    var aux: bool;
-    var aux_0: W64.t;
-    
-    var x:W64.t Array4.t;
     var t:W64.t Array4.t;
-    var twop63:W64.t;
+    var z:W64.t Array4.t;
     var cf:bool;
+    var r1:W64.t;
+    var r2:W64.t;
     t <- witness;
-    x <- witness;
-    x.[0] <- xx.[0];
-    x.[1] <- xx.[1];
-    x.[2] <- xx.[2];
-    x.[3] <- xx.[3];
-    t <-  x;
-    twop63 <- (W64.of_int 1);
-    twop63 <- (twop63 `<<` (W8.of_int 63));
-    (aux, aux_0) <- addc_64 t.[0] (W64.of_int 19) false;
-    cf <- aux;
-    t.[0] <- aux_0;
-    (aux, aux_0) <- addc_64 t.[1] (W64.of_int 0) cf;
-    cf <- aux;
-    t.[1] <- aux_0;
-    (aux, aux_0) <- addc_64 t.[2] (W64.of_int 0) cf;
-    cf <- aux;
-    t.[2] <- aux_0;
-    (aux, aux_0) <- addc_64 t.[3] twop63 cf;
-    cf <- aux;
-    t.[3] <- aux_0;
-    x.[0] <- (cf ? t.[0] : x.[0]);
-    x.[1] <- (cf ? t.[1] : x.[1]);
-    x.[2] <- (cf ? t.[2] : x.[2]);
-    x.[3] <- (cf ? t.[3] : x.[3]);
-    xx.[0] <- x.[0];
-    xx.[1] <- x.[1];
-    xx.[2] <- x.[2];
-    xx.[3] <- x.[3];
-    return (xx);
+    z <- witness;
+    z.[0] <- x.[0];
+    z.[1] <- x.[1];
+    z.[2] <- x.[2];
+    z.[3] <- x.[3];
+    (cf, t) <@ bn_subc (z, p);
+    r1 <- t.[0];
+    r2 <- x.[0];
+    r1 <- (cf ? r2 : r1);
+    t.[0] <- r1;
+    r1 <- t.[1];
+    r2 <- x.[1];
+    r1 <- (cf ? r2 : r1);
+    t.[1] <- r1;
+    r1 <- t.[2];
+    r2 <- x.[2];
+    r1 <- (cf ? r2 : r1);
+    t.[2] <- r1;
+    r1 <- t.[3];
+    r2 <- x.[3];
+    r1 <- (cf ? r2 : r1);
+    t.[3] <- r1;
+    return (t);
   }
   
-  proc redp25519 (_of:bool, _cf:bool, a:W64.t Array8.t) : W64.t Array4.t = {
-    
-    var al:W64.t Array4.t;
-    var tmp:W64.t;
-    var _zero:W64.t;
-    var ah:W64.t Array4.t;
-    var  _0:W64.t Array4.t;
-    var  _1:bool;
-    var  _2:bool;
-    var  _3:bool;
-    var  _4:bool;
-    var  _5:bool;
-    var  _6:W64.t Array4.t;
-     _0 <- witness;
-     _6 <- witness;
-    ah <- witness;
-    al <- witness;
-    tmp <- (W64.of_int 38);
-    _zero <- (W64.of_int 0);
-    (ah,  _0) <@ bn2_unpack (a);
-    (_zero, _of, _cf, a) <@ mul1acc (0, tmp, ah, a, _zero, _of, _cf);
-    ( _1,  _2,  _3,  _4,  _5, tmp) <- IMULri_64 a.[4] (W64.of_int 38);
-    ( _6, al) <@ bn2_unpack (a);
-    (_cf, al) <@ bn_add1 (al, tmp);
-    tmp <@ maskOnCarry (38, tmp, _cf);
-    al.[0] <- (al.[0] + tmp);
-    return (al);
-  }
-  
-  proc freeze (x:W64.t Array4.t) : W64.t Array4.t = {
-    
-    
-    
-    x <@ cminusP (x);
-    x <@ cminusP (x);
-    return (x);
-  }
-  
-  proc mulm (p:W64.t Array4.t, f:W64.t Array4.t, g:W64.t Array4.t) : 
+  proc addm (p:W64.t Array4.t, a:W64.t Array4.t, b:W64.t Array4.t) : 
   W64.t Array4.t = {
     
-    var _zero:W64.t;
-    var of_0:bool;
-    var cf:bool;
-    var h:W64.t Array8.t;
-    h <- witness;
-    (_zero, of_0, cf, h) <@ bn_muln (f, g);
-    g <@ redp25519 (of_0, cf, h);
-    g <@ freeze (g);
-    return (g);
-  }
-  
-  proc addm (a:W64.t Array4.t, b:W64.t Array4.t) : W64.t Array4.t = {
-    
     var f:W64.t Array4.t;
+    var z:W64.t Array4.t;
     var  _0:bool;
     f <- witness;
+    z <- witness;
     ( _0, f) <@ bn_addc (a, b);
-    f <@ cminusP (f);
+    z.[0] <- f.[0];
+    z.[1] <- f.[1];
+    z.[2] <- f.[2];
+    z.[3] <- f.[3];
+    f <@ cminusP (p, z);
     return (f);
   }
   
-  proc expm (m:W64.t Array4.t, x:W64.t Array4.t, n:W64.t Array4.t) : 
+  proc mulm (m:W64.t Array4.t, x:W64.t Array4.t, n:W64.t Array4.t) : 
   W64.t Array4.t = {
     
     var x1:W64.t Array4.t;
@@ -362,17 +179,20 @@ module M = {
     x3 <- witness;
     x4 <- witness;
     ctr <- (W64.of_int ((4 * 64) - 1));
-    x1.[0] <- (W64.of_int 1);
+    x1.[0] <- (W64.of_int 0);
     x1.[1] <- (W64.of_int 0);
     x1.[2] <- (W64.of_int 0);
     x1.[3] <- (W64.of_int 0);
-    x2.[0] <- (W64.of_int 1);
+    x2.[0] <- (W64.of_int 0);
     x2.[1] <- (W64.of_int 0);
     x2.[2] <- (W64.of_int 0);
     x2.[3] <- (W64.of_int 0);
     d <@ ith_bit (n, ctr);
-    x3 <- x;
-    x4 <@ mulm (m, x, x);
+    x3.[0] <- x.[0];
+    x3.[1] <- x.[1];
+    x3.[2] <- x.[2];
+    x3.[3] <- x.[3];
+    x4 <@ addm (m, x, x);
     p <- d;
     (x1, x3) <@ swapr (x1, x3, d);
     (x2, x4) <@ swapr (x2, x4, d);
@@ -387,8 +207,8 @@ module M = {
       d <- (d `|` t2);
       par <- (t1 `^` t2);
       (x1, x2) <@ swapr (x1, x2, par);
-      x1 <@ mulm (m, x1, x2);
-      x2 <@ mulm (m, x2, x2);
+      x1 <@ addm (m, x1, x2);
+      x2 <@ addm (m, x2, x2);
       q <- (q `|` t2);
       cbit <- (q `^` p);
       (x1, x3) <@ swapr (x1, x3, cbit);
@@ -401,6 +221,7 @@ module M = {
   
   proc toEC () : unit = {
     
+    var p:W64.t Array4.t;
     var a:W64.t Array4.t;
     var b:W64.t Array4.t;
     var r:W64.t Array4.t;
@@ -409,10 +230,10 @@ module M = {
      _0 <- witness;
     a <- witness;
     b <- witness;
+    p <- witness;
     r <- witness;
-    r <@ addm (a, b);
-    r <@ mulm (a, a, b);
-    r <@ expm (a, a, b);
+    r <@ addm (p, a, b);
+    r <@ mulm (p, a, b);
     x <@ ith_bit (a, x);
     ( _0, a) <@ swapr (a, a, x);
     return ();
