w64x4/src/Array8.ec
@@ -1,3 +1,3 @@
-from Jasmin require import JArray.
+ require import JArray.
 
 clone export PolyArray as Array8  with op size <- 8.
